LambdaS5/coq/LibFinset.v
@@ -6,7 +6,7 @@
 Set Implicit Arguments.
 Require Import LibTactics LibList.
 Require Import LibSet LibLogic LibEqual LibReflect LibOrder.
-Generalizable Variable A.
+Generalizable Variables A U.
 
 (** DISCLAIMER: for the time being, this file only contains the
     operations for type fset, but not yet all the typeclasses 
@@ -15,153 +15,210 @@ Generalizable Variable A.
 
 (* ********************************************************************** *)
 (** * Abstract interface for finite sets *)
-(*
-Module Type FsetSig.
+
+Module Type FinsetSig.
 
 (** Definitions and operations on finite sets *)
 
-Section Operations.
+Section Definitions.
 Variables (A:Type).
 
-Parameter fset : Type -> Type.
+Parameter finset : Type -> Type.
 
-Parameter to_list : fset A -> list A.
-Parameter from_list : list A -> fset A.
+Parameter to_list : finset A -> list A.
+Parameter from_list : list A -> finset A.
 
-End Operations.
-
-(** Notations *)
-
-Section Properties.
-Variables A : Type.
-Implicit Types x : A.
-Implicit Types E : fset A.
-
-Parameter union_inst : Comparable A -> BagUnion (fset A).
-Parameter inter_inst : Comparable A -> BagInter (fset A).
-Parameter remove_inst : Comparable A -> BagRemove (fset A) (fset A).
-Parameter empty_inst : Comparable A -> BagEmpty (fset A).
-Parameter in_inst : Comparable A -> BagIn A (fset A).
-Parameter single_inst : Comparable A -> BagSingle A (fset A).
-Parameter incl_inst : Comparable A -> BagIncl (fset A).
-Parameter disjoint_inst : Comparable A -> BagDisjoint (fset A).
-
-Existing Instances union_inst inter_inst remove_inst empty_inst in_inst
-    single_inst incl_inst disjoint_inst.
+Parameter in_impl : A -> finset A -> Prop.
+Parameter empty_impl : finset A.
+Parameter single_impl : A -> finset A.
+Parameter union_impl : finset A -> finset A -> finset A.
+Parameter inter_impl : finset A -> finset A -> finset A.
+Parameter remove_impl : finset A -> finset A -> finset A.
+Parameter incl_impl : finset A -> finset A -> Prop.
+Parameter disjoint_impl : finset A -> finset A -> Prop.
+Parameter card_impl : finset A -> nat.
 
 (** Extensionality *)
 
-Parameter fset_extens : forall (cmp : Comparable A) (E : fset A) (F : fset A), 
-  E \c F -> F \c E -> E = F.
+Parameter extens_impl : forall E E', 
+  incl_impl E E' -> incl_impl E' E -> E = E'.
 
 (** Semantics of basic operations *)
 
-Parameter in_empty_eq_inst : forall (cmp : Comparable A), In_empty_eq.
-Parameter in_single_eq_inst : forall (cmp : Comparable A), In_single_eq.
-Parameter in_union_eq_inst : forall (cmp : Comparable A), In_union_eq.
-Parameter in_inter_eq_inst : forall (cmp : Comparable A), In_inter_eq.
-Parameter in_remove_eq_inst : forall (cmp : Comparable A), In_remove_eq.
+Parameter in_empty_eq_impl : forall x, in_impl x empty_impl = False.
+Parameter in_single_eq_impl : forall x y, in_impl x (single_impl y) = (x = y).
+Parameter in_union_eq_impl : forall x E1 E2, in_impl x (union_impl E1 E2) = (in_impl x E1 \/ in_impl x E2).
+Parameter in_inter_eq_impl : forall x E1 E2, in_impl x (inter_impl E1 E2) = (in_impl x E1 /\ in_impl x E2).
+Parameter in_remove_eq_impl : forall x E1 E2, in_impl x (remove_impl E1 E2) = (in_impl x E1 /\ ~in_impl x E2).
 
-Existing Instances in_empty_eq_inst in_single_eq_inst in_union_eq_inst
-    in_inter_eq_inst in_remove_eq_inst.
+Parameter mem_decidable : forall (s : finset A) x, Decidable (in_impl x s).
 
-Parameter mem_decidable : forall (cmp : Comparable A) (s:fset A) x,
-   Decidable (x \in s).
-Existing Instances mem_decidable.
+End Definitions.
 
-End Properties.
-
-End FsetSig.
-
-Print Module Type FsetSig.
+End FinsetSig.
 
 (* ********************************************************************** *)
 (** * Implementation of finite sets *)
 
-Module Export FsetImpl : FsetSig.
-*)
-(** Note: most of the material contained in this module will ultimately
-    be moved into the TLC library in a file called LibFset. *)
-
-Definition finset A := list A.
+Module Export FinsetImpl : FinsetSig.
 
 Section Operations.
 Variables (A:Type).
- 
-Definition from_list (L : list A) : finset A := L.
 
-Definition to_list (E : finset A) : list A := E.
+Definition finite (U : set A) :=
+  exists L, forall x, x \in U -> Mem x L.
 
-End Operations.
+Definition finset := sig finite.
 
-(** Notations *)
-
-Section Properties.
-Variables A : Type.
 Implicit Types x : A.
-Implicit Types E : finset A.
+Implicit Types E : finset.
 
-Global Instance union_inst : Comparable A -> BagUnion (finset A) :=
-  { union := fun E F => E ++ List.filter (fun x => !LibList.mem_decide x E) F }. 
+Definition build_fset `(F:finite U) : finset := exist finite U F.
 
-Global Instance inter_inst : Comparable A -> BagInter (finset A) :=
-  { inter := fun E F => List.filter (fun x => LibList.mem_decide x F) E }.
+Lemma finite_empty : finite \{}.
+Proof. exists (@nil A). intros x. rewrite in_empty_eq. auto_false. Qed.
 
-Global Instance remove_inst : Comparable A -> BagRemove (finset A) (finset A) :=
-  { remove := fun E F => List.filter (fun x => !LibList.mem_decide x F) E }.
-
-Global Instance empty_inst : Comparable A -> BagEmpty (finset A) := 
-  { empty := nil }.
-
-Global Instance in_inst : Comparable A -> BagIn A (finset A) :=
-  { is_in := fun x E => LibList.Mem x E }.
-
-Global Instance single_inst : Comparable A -> BagSingle A (finset A) := 
-  { single := fun x => x :: nil }.
-
-Global Instance incl_inst : Comparable A -> BagIncl (finset A) :=
-  { incl := fun E F => forall x, x \in E -> x \in F }.
-
-Global Instance disjoint_inst : Comparable A -> BagDisjoint (finset A) :=
-  { disjoint := fun E F => inter E F = empty }.
-
-Lemma finset_extens_eq : forall (cmp : Comparable A) (E : finset A) F,
-  (forall x, x \in E = x \in F) -> E = F.
+Lemma singleton_finite : forall x, finite \{x}.
 Proof.
-(* TODO *)
+  intros. exists (x::nil). intros y. 
+  rewrite in_single_eq. intro_subst. constructor.
+Qed.
+
+Lemma union_finite : forall U V : set A,
+  finite U -> finite V -> finite (U \u V).
+Proof.
+  introv [L1 E1] [L2 E2]. exists (L1 ++ L2). intros x.
+  rewrite in_union_eq. rewrite Mem_app_or_eq. introv [H|H]; auto. 
+Qed.
+
+Lemma inter_finite : forall U V : set A,
+  finite U -> finite V -> finite (U \n V).
+Proof.
+  introv [L1 E1] [L2 E2]. exists (L1 ++ L2). intros x.
+  rewrite in_inter_eq. rewrite Mem_app_or_eq. auto*.
+Qed.
+
+Lemma remove_finite : forall U V : set A,
+  finite U -> finite V -> finite (U \- V).
+Proof.
+  introv [L1 E1] [L2 E2]. exists L1. intros x.
+  rewrite in_remove_eq. introv [H1 H2]; auto. 
+Qed.
+
+Definition in_impl x E := x \in proj1_sig E.
+Definition empty_impl := build_fset finite_empty.
+Definition single_impl x := build_fset (singleton_finite x). 
+Definition union_impl E E' := build_fset (union_finite (proj2_sig E) (proj2_sig E')).
+Definition inter_impl E E' := build_fset (inter_finite (proj2_sig E) (proj2_sig E')).
+Definition remove_impl E E' := build_fset (remove_finite (proj2_sig E) (proj2_sig E')).
+Definition incl_impl E E' := forall x, in_impl x E -> in_impl x E'.
+Definition disjoint_impl E E' := inter_impl E E' = empty_impl.
+
+Definition listish (U : set A) :=
+  exists L, forall x, is_in x U = Mem x L.
+
+Lemma finite_listish : forall U, finite U -> listish U.
+Proof.
 Admitted.
 
-Lemma finset_extens : forall (cmp : Comparable A) (E : finset A)  F, 
-  E \c F -> F \c E -> E = F.
-Proof. intros. applys finset_extens_eq. extens*. Qed.
+Definition from_list (L : list A) : finset := 
+  fold_right (fun x acc => union_impl (single_impl x) acc) empty_impl L.
 
-Global Instance in_empty_eq_inst : forall (cmp : Comparable A), In_empty_eq (A:=A) (T:=finset A).
-Proof. constructor. simpl. intros. apply Mem_nil_eq. Qed.
+Definition to_list E : list A := 
+  proj1_sig (indefinite_description (finite_listish (proj2_sig E))).
 
-Global Instance in_single_eq_inst : forall (cmp : Comparable A), In_single_eq (A:=A) (T:=finset A).
-Proof. constructor. simpl. intros. rewrite Mem_cons_eq. rewrite Mem_nil_eq. rew_logic*. Qed.
+Definition card_impl E := length (to_list E).
 
-Global Instance in_union_eq_inst : forall (cmp : Comparable A), In_union_eq (A:=A) (T:=finset A).
-Proof. Admitted.
-
-Global Instance in_inter_eq_inst : forall (cmp : Comparable A), In_inter_eq (A:=A) (T:=finset A).
-Proof. Admitted.
-
-Global Instance in_remove_eq_inst : forall (cmp : Comparable A), In_remove_eq (A:=A) (T:=finset A).
-Proof. Admitted.
-
-Lemma mem_decidable : forall (cmp : Comparable A) (s:finset A) x,
-   Decidable (x \in s).
+Lemma extens_eq_impl : forall E F,
+  (forall x, in_impl x E = in_impl x F) -> E = F.
 Proof.
-  intros. applys decidable_make (LibList.mem_decide x s).
-  skip.
+  unfold mem. intros [U FU] [V FV] H. simpls.
+  apply exist_eq. apply in_double_eq. auto.
+Qed. 
+
+Lemma extens_impl : forall E F,
+  incl_impl E F -> incl_impl F E -> E = F.
+Proof. intros. apply extens_eq_impl. extens*. Qed.
+
+Lemma in_empty_eq_impl : forall x, in_impl x empty_impl = False.
+Proof. unfold in_impl, empty_impl. simpl. intros. rewrite in_empty_eq. auto*. Qed.
+
+Lemma in_single_eq_impl : forall x y, in_impl x (single_impl y) = (x = y).
+Proof. unfold in_impl, single_impl. simpl. intros. rewrite in_single_eq. auto*. Qed.
+
+Lemma in_union_eq_impl : forall x E1 E2, in_impl x (union_impl E1 E2) = (in_impl x E1 \/ in_impl x E2).
+Proof. unfold in_impl, union_impl. simpl. intros. rewrite in_union_eq. auto*. Qed.
+
+Lemma in_inter_eq_impl : forall x E1 E2, in_impl x (inter_impl E1 E2) = (in_impl x E1 /\ in_impl x E2).
+Proof. unfold in_impl, inter_impl. simpl. intros. rewrite in_inter_eq. auto*. Qed.
+
+Lemma in_remove_eq_impl : forall x E1 E2, in_impl x (remove_impl E1 E2) = (in_impl x E1 /\ ~in_impl x E2).
+Proof. unfold in_impl, remove_impl. simpl. intros. rewrite in_remove_eq. auto*. Qed.
+
+Lemma mem_decidable : forall E x,
+   Decidable (in_impl x E).
+Proof.
+skip.
 Defined.
 
-End Properties.
-(*
-End FsetImpl.
-*)
+End Operations.
+End FinsetImpl.
 
+Global Instance union_inst : BagUnion (finset A) :=
+  { union := @FinsetImpl.union_impl _ }.
+
+Global Instance inter_inst : BagInter (finset A) :=
+  { inter := @FinsetImpl.inter_impl _ }.
+
+Global Instance remove_inst : BagRemove (finset A) (finset A) :=
+  { remove := @FinsetImpl.remove_impl _ }.
+
+Global Instance empty_inst : BagEmpty (finset A) := 
+  { empty := @FinsetImpl.empty_impl _ }.
+
+Global Instance in_inst : BagIn A (finset A) :=
+  { is_in := @FinsetImpl.in_impl _ }.
+
+Global Instance single_inst : BagSingle A (finset A) := 
+  { single := @FinsetImpl.single_impl _ }.
+
+Global Instance incl_inst : BagIncl (finset A) :=
+  { incl := @FinsetImpl.incl_impl _ }.
+
+Global Instance disjoint_inst : BagDisjoint (finset A) :=
+  { disjoint := @FinsetImpl.disjoint_impl _ }.
+
+Global Instance card_inst : BagCard (finset A) :=  
+  { card := @FinsetImpl.card_impl _ }.
+
+Global Instance in_empty_eq_inst : In_empty_eq (T := finset A) :=
+  { in_empty_eq := @FinsetImpl.in_empty_eq_impl _ }.
+
+Global Instance in_single_eq_inst : In_single_eq (T := finset A) :=
+  { in_single_eq := @FinsetImpl.in_single_eq_impl _ }.
+
+Global Instance in_union_eq_inst : In_union_eq (T := finset A) :=
+  { in_union_eq := @FinsetImpl.in_union_eq_impl _ }.
+
+Global Instance in_inter_eq_inst : In_inter_eq (T := finset A) :=
+  { in_inter_eq := @FinsetImpl.in_inter_eq_impl _ }.
+
+Global Instance in_remove_eq_inst : In_remove_eq (T := finset A) :=
+  { in_remove_eq := @FinsetImpl.in_remove_eq_impl _ }.
+
+Global Opaque union_inst inter_inst remove_inst empty_inst in_inst
+    single_inst incl_inst disjoint_inst.
+
+Extraction Language Ocaml.
+
+Extract Constant FinsetImpl.finset "'A" => "'A BatSet.t". 
+Extract Constant FinsetImpl.from_list => "fun l -> BatSet.of_list l".
+Extract Constant FinsetImpl.to_list => "fun s -> BatSet.to_list s".
+Extract Constant FinsetImpl.empty_impl => "BatSet.empty".
+Extract Constant FinsetImpl.single_impl => "fun x -> BatSet.singleton x".
+Extract Constant FinsetImpl.union_impl => "fun s1 s2 -> BatSet.union s1 s2".
+Extract Constant FinsetImpl.inter_impl => "fun s1 s2 -> BatSet.intersect s1 s2".
+Extract Constant FinsetImpl.remove_impl => "fun s1 s2 -> BatSet.diff s1 s2".
 
 (* ********************************************************************** *)
 (** * Derivable properties about finite sets *)
